Makefile
@@ -19,7 +19,6 @@ SRCS = \
 	   src/SDK/CMM/DefaultCMM.dfy \
 	   src/SDK/CMM/Defs.dfy \
 	   src/SDK/Keyring/AESKeyring.dfy \
-	   src/SDK/Keyring/AESWrappingSuite.dfy \
 	   src/SDK/Keyring/Defs.dfy \
 	   src/SDK/Keyring/RSAKeyring.dfy \
 	   src/SDK/Materials.dfy \
